WIP

FlowEquivalence.v
@@ -34,7 +34,7 @@ Open Scope list_scope.
   | [] => false
   | b :: ls' => if dec a b then true else in_list_dec a ls'
   end.
-  Infix "∈" := in_list_dec (no associativity, at level 90).
+  Notation "a ∈ ls" := (in_list_dec a ls = true) (no associativity, at level 90).
 
 
 
@@ -124,23 +124,23 @@ Section LatchSequence.
 
 
   Inductive latch_sequence : kind -> Set :=
-  | ls_empty_sync : CLK -> latch_sequence Sync
+  | ls_empty_sync : (*CLK ->*) latch_sequence Sync
   | ls_empty_async : latch_set -> latch_sequence Async
   | ls_async (e : event)
              (next : latch_sequence Async)
            : latch_sequence Async
-  | ls_sync (clk : CLK)
+  | ls_sync (*clk : CLK*)
             (next : latch_sequence Sync)
            : latch_sequence Sync
   .
 
   Fixpoint is_transparent {k} (s : latch_sequence k) : latch_set :=
     match s with
-    | ls_empty_sync CLK0 => is_even
-    | ls_empty_sync CLK1 => is_odd
+(*    | ls_empty_sync => is_even*)
+    | ls_empty_sync   => fun _ => false (*is_odd*)
     | ls_empty_async ls  => ls
-    | ls_sync CLK0 _ => is_even
-    | ls_sync CLK1 _ => is_odd
+    | ls_sync _ => fun _ => false (*is_even*)
+(*    | ls_sync _ => (*is_odd*)*)
     | ls_async e s' => step_latch_set e (is_transparent s')
     end.
 
@@ -154,10 +154,10 @@ Section LatchSequence.
 
   Definition step_latch_sequence {k} (s : latch_sequence k) : latch_sequence k :=
     match s with
-    | ls_empty_sync clk => ls_empty_sync (step_CLK clk)
+    | ls_empty_sync => ls_empty_sync
     | ls_empty_async ls => ls_empty_async ls
     | ls_async ls s' => s'
-    | ls_sync clk s' => s'
+    | ls_sync s' => s'
     end.
 
   Fixpoint step_latch_sequence_n {k} (s : latch_sequence k) (n : nat)
@@ -198,25 +198,21 @@ Section LatchSequence.
     | Neg _, false => false
     end.
 
-  (* Returns the number of timesteps at which the event will occur. Will never
-  return Some 0. *)
+  (* Returns the number of timesteps at which the event will occur. *)
   Fixpoint find_next_occurrence {k} (e : event) (s : latch_sequence k)
                               : option nat :=
   match s with
-  | ls_empty_sync _ => None
+  | ls_empty_sync    => None
   | ls_empty_async _ => None
-  | ls_sync CLK0 _ => match e with
-                      | Pos _ => (* The even l+ will occur when the clock goes
-                                    high, so on the next time step. *)
-                                 Some 1
-                      | Neg _ => Some 2
-                      end
+  | ls_sync _ => Some 1
+(*
   | ls_sync CLK1 _ => match e with
                       | Pos _ => (* The even l+ will occur when the clock goes
                                     high *)
                                  Some 2
                       | Neg _ => Some 1
                       end
+*)
   | ls_async e0 s' => if eqb e e0
                       then Some 1
                       else fmap S (find_next_occurrence e s')
@@ -240,7 +236,9 @@ Arguments ls_empty_async {even odd}.
 Arguments ls_async {even odd}.
 Arguments ls_sync {even odd}.
 
-
+About Pos.
+Arguments Pos {even odd}.
+Arguments Neg {even odd}.
 
 (*************)
 (** Circuits *)
@@ -262,9 +260,9 @@ Section Circuits.
 
   Record circuit : Set :=
   { even_odd_neighbors : list (even * odd)
-  ; evenF : forall (e : even), state {o : odd & In (e,o) even_odd_neighbors} -> value
   ; odd_even_neighbors : list (odd * even)
-  ; oddF : forall (o : odd), state {e : even & In (o,e) odd_even_neighbors} -> value
+  ; evenF : forall (e : even), state {o : odd & In (o,e) odd_even_neighbors} -> value
+  ; oddF : forall (o : odd), state {e : even & In (e,o) even_odd_neighbors} -> value
   }.
 
 (*
@@ -291,6 +289,56 @@ Section Circuits.
     | Odd o  => oddF c o (even_state _ prev)
     end.
 
+  Definition transparent_event (l : latch even odd) : event even odd :=
+    match l with
+    | Even e => Neg (Even e)
+    | Odd o  => Pos (Odd o)
+    end.
+  Definition opaque_event (l : latch even odd) : event even odd :=
+    match l with
+    | Even e => Pos (Even e)
+    | Odd o  => Neg (Odd o)
+    end.
+    
+
+
+Print latch_sequence. Print is_transparent. Print step_latch_set.
+
+
+  (* step odd latches *)
+  Definition eval_sync_odd_1 (c : circuit) (prev : state (latch even odd))
+                      : state (latch even odd) :=
+    fun l => match l with
+             | Odd o => get_latch_value c prev (Odd o)
+             | _ => prev l
+             end.
+  (* step even latches *)
+  Existing Instance event_eq_dec.
+  Definition eval_sync_even_1 (c : circuit) (prev : state (latch even odd))
+                             : state (latch even odd) :=
+    fun l => match l with
+             | Even e => get_latch_value c prev (Even e)
+             | _ => prev l
+             end. 
+  Definition eval_async_1 (c : circuit) (prev : state (latch even odd)) (e : event even odd) 
+                        : state (latch  even odd) :=
+    fun l => if transparent_event l =? e (*event_refers_to_latch even odd e l && event_becomes_transparent _ _ e*)
+             then get_latch_value c prev l
+             else prev l.
+
+  Fixpoint eval {k} (c : circuit) (prev : state (latch even odd))
+                (s : latch_sequence even odd k)
+                : state (latch even odd) :=
+    match s with
+    | ls_empty_sync       => prev
+    | ls_empty_async lset => prev
+    | ls_sync s'          => let st := eval c prev s' in
+                             eval_sync_even_1 c (eval_sync_odd_1 c st)
+    | ls_async e s'       => let st := eval c prev s' in
+                             eval_async_1 c st e s'
+    end.
+
+(*
   Definition eval_latch_sequence_1 {k : kind} 
                                    (c : circuit)
                                    (prev : state (latch even odd))
@@ -308,7 +356,7 @@ Section Circuits.
   | 0 => init
   | S n' => eval_latch_sequence_1 c (eval c init s n') s
   end.
-
+*)
 (*
   Fixpoint repeat {A} (n : nat) (ls : list A) : list A :=
     match n with
@@ -320,6 +368,8 @@ Section Circuits.
 End Circuits.
 
 Arguments eval {even odd Heven Hodd k}.
+Arguments transparent_event {even odd}.
+Arguments opaque_event {even odd}.
 
 
 Class Enumerable (A : Set) :=
@@ -348,7 +398,7 @@ Section MarkedGraphs.
     fmap (fun ete => (snd (fst ete),snd ete)) (input_event_output M).
 
   Definition in_transitions (M : marked_graph) (e : events) : list transitions :=
-    let f := fun ete => if fst (fst ete) =? e then [snd (fst ete)] else [] in
+    let f := fun ete => if snd ete =? e then [snd (fst ete)] else [] in
     flat_map f (input_event_output M).
 (*
   Definition in_transitions (M : marked_graph) (e : events) : list transitions :=
@@ -363,7 +413,12 @@ Section MarkedGraphs.
 
 
   Instance prod_eq_dec {A B} `{eq_dec A} `{eq_dec B} : eq_dec (A*B).
-  Admitted.
+  Proof.
+    split. intros [a b] [a' b'].
+    destruct (dec a a'); destruct (dec b b');
+      subst; auto;
+      right; inversion 1; contradiction.
+  Defined.
 
   (* An event should only fire if the caller has independently checked that it
   is enabled. *) 
@@ -423,6 +478,7 @@ Arguments traces {events transitions} {Hevents Htransitions}.
 Arguments step_latch_sequence {even odd k}.
 Arguments step_latch_sequence_n {even odd k}.
 Arguments find_ith_occurrence {even odd Heven Hodd k}.
+Arguments fire {events transitions Hevents Htransitions}.
 
 Section FlowEquivalence.
 
@@ -437,11 +493,25 @@ Section FlowEquivalence.
 (*  Context `{Enumerable transitions}. *)
 
   Existing Instance event_eq_dec.
-  Definition isEnabled (e : event even odd) (m : marking transitions) : Prop :=
+
+  Definition is_enabled (e : event even odd) (m : marking transitions) : Prop :=
     enabled e M m = true.
 
-  Record marking_consistent_with_latch_sequence {k}
-         (m : marking transitions) (s : latch_sequence even odd k) :=
+About fire.
+  Inductive ls_consistent_with_MG : latch_sequence even odd Async -> marking transitions -> Prop :=
+  | lsc_empty lset : ls_consistent_with_MG (ls_empty_async lset) init
+  | lsc_cons e m m' s' : is_enabled e m ->
+                fire e M m = m' ->
+                ls_consistent_with_MG s' m ->
+                ls_consistent_with_MG (ls_async e s') m'
+  .
+
+  Definition consistent (s : latch_sequence even odd Async) : Prop := exists m, ls_consistent_with_MG s m.
+    
+(*
+Print is_transparent.
+  Record marking_consistent_with_latch_sequence
+         (m : marking transitions) (s : latch_sequence even odd Async) :=
     { PosEvenEnabled : forall (e : even),
                        isEnabled (Pos (Even e)) m -> is_transparent s (Even e) = true
     ; NegEvenEnabled : forall (e : even),
@@ -452,11 +522,14 @@ Section FlowEquivalence.
                       isEnabled (Neg (Odd o)) m -> is_transparent s (Odd o) = true
     }.
 
-  Definition consistent_with_MG {k} (s : latch_sequence even odd k) :=
+  Definition consistent_with_MG (s : latch_sequence even odd Async) :=
+    
+
     forall (trace : nat -> marking transitions),
       traces M trace ->
       forall i,
         marking_consistent_with_latch_sequence (trace i) (step_latch_sequence_n s i).
+*)
 
   (* An initial marking indicates an initial state in that for each latch l, if
   l+ is enabled first, then l=0, and if l- is enabled first, then l=1. *)
@@ -466,11 +539,6 @@ Section FlowEquivalence.
              else X.
 (*  Definition init_state := marking_to_state init.*)
 
-  Definition transparent_event (l : latch even odd) : event even odd :=
-    match l with
-    | Even e => Neg (Even e)
-    | Odd o  => Pos (Odd o)
-    end.
 
 Print latch_sequence. Print eval. Search CLK.
 
@@ -482,19 +550,57 @@ Print latch_sequence. Print eval. Search CLK.
     | _, _  => false
     end.
 
-  Search state. Print eval_latch_sequence_1. 
-Arguments eval_latch_sequence_1 {even odd Heven Hodd k}.
+  Search state. 
+(*Arguments eval_latch_sequence_1 {even odd Heven Hodd k}.*)
 
-Print get_latch_value.
+Print get_latch_value. About eval.
+Print kind.
 
 
+  Fixpoint ls_length {k} (s : latch_sequence even odd k) : nat :=
+    match s with
+    | ls_empty_sync => 0
+    | ls_empty_async _ => 0
+    | ls_async _ s' => 1 + ls_length s'
+    | ls_sync s' => 1 + ls_length s'
+    end.
+
+  Print eval.
+
+  
+
+  Fixpoint sync_eval (c : circuit even odd) (st : state (latch even odd)) (n : nat) :=
+    match n with
+    | 0 => st
+    | S n' => let st' := sync_eval c st n' in
+              fun l => get_latch_value _ _ c st' l
+    end.
+
+  Fixpoint num_events (e : event even odd) (s : latch_sequence even odd Async) : nat :=
+    match s with
+    | ls_empty_async _ => 0
+    | ls_async e' s' => if e =? e'
+                        then 1 + num_events e s'
+                        else num_events e s'
+    end.
+
+
+  Definition flow_equivalence (c : circuit even odd) :=
+    forall (s : latch_sequence even odd Async),
+(*      ls_consistent_with_MG s init ->*)
+        consistent s ->
+        eval c (marking_to_state init) s
+      = fun l => sync_eval c (marking_to_state init) (num_events (opaque_event l) s) l.
+
+(*
   Fixpoint projection {k} (c : circuit even odd) (s : latch_sequence even odd k)
                           (l : latch even odd)
                           (old_st : state (latch even odd))
                           (i : nat) (* the ith value latched by l *) 
                        :  value :=
+
     match s with
-    | ls_empty_sync _ => old_st l
+    | ls_empty_sync => old_st l
     | ls_empty_async lset => old_st l
     | ls_async e s' => match i with
                        | 0    => old_st l
@@ -502,9 +608,13 @@ Print get_latch_value.
                                  then projection c s' l (eval_latch_sequence_1 c old_st s) i'
                                  else projection c s' l (eval_latch_sequence_1 c old_st s) (S i')
                        end
-    | ls_sync clk s' => match i with
-                        | 0 => old_st l
-                        | S i' => if transparent_on_clock l clk
+    | ls_sync s' => eval c old_st s' 
+
+match i with
+                    | 0 => old_st l
+                    | S i' => 
+
+if transparent_on_clock l clk
                                   then projection c s' l (eval_latch_sequence_1 c old_st s) i'
                                   else projection c s' l (eval_latch_sequence_1 c old_st s) (S i')
                         end
@@ -533,28 +643,11 @@ Print get_latch_value.
                 end
       end.
 *)
-
-  Fixpoint ls_length {k} (s : latch_sequence even odd k) : nat :=
-    match s with
-    | ls_empty_sync _ => 0
-    | ls_empty_async _ => 0
-    | ls_async _ s' => 1 + ls_length s'
-    | ls_sync _ s' => 1 + ls_length s'
-    end.
-
-  Fixpoint sync_latch_sequence (n : nat) (clk : CLK) : latch_sequence even odd Sync :=
-    match n with
-    | 0 => ls_empty_sync clk
-    | S n' => ls_sync clk (sync_latch_sequence n' (step_CLK clk))
-    end.
-
-  Definition flow_equivalence (c : circuit even odd) (init_clk : CLK) :=
-    forall (s : latch_sequence even odd Async),
-      consistent_with_MG s ->
-      forall (l : latch even odd) (i : nat),
-        projection c s l (marking_to_state init) i 
-      = projection c (sync_latch_sequence (ls_length s) init_clk) l (marking_to_state init) i.
+*)
 
 End FlowEquivalence.
 
+
 Arguments flow_equivalence {even odd Heven Hodd transitions Htrans}.
+Arguments marking_to_state {even odd Heven Hodd transitions}.
+Arguments sync_eval {even odd} c. 
