Monad.v
@@ -1,0 +1,396 @@
+Require Import List.
+Require Import Program.
+
+(** ** Type Classes for functors, applicatives, and monads *)
+
+Local Notation "f ∘ g" := (fun x => f (g x)) (at level 40, left associativity).
+
+Class Functor (f : Type -> Type) : Type :=
+  { fmap         : forall {A B}, (A -> B) -> f A -> f B }. 
+Class Applicative (f : Type -> Type) `{F : Functor f} : Type :=
+  { pure : forall {A}, A -> f A;
+    liftA : forall {A B}, f (A -> B) -> f A -> f B
+  }.
+Class Monad (m: Type -> Type) `{M : Applicative m} : Type :=
+  { bind: forall {A}, m A -> forall {B}, (A -> m B) -> m B
+  }.
+Definition return_ {m : Type -> Type} `{M : Monad m} {A : Type} : A -> m A := pure.
+
+(** ** Notations *)
+
+Module Notations.
+  Notation "f <*> a" := (liftA f a) (left associativity, at level 64) : monad_scope.
+  Notation "a >>= f" := (bind a f)  (left associativity, at level 66) : monad_scope.
+  Notation "a >> b" := (bind a (fun _ => b)) (at level 66, left associativity) : monad_scope.
+  Notation "'do' a ← e ; c" := (bind e (fun a => c)) (at level 80, right associativity) : monad_scope.
+  Notation "'do' ( a , b ) ← e ; c" := (bind e (fun x => let (a,b) := x in c)) (at level 80, right associativity) : monad_scope.
+End Notations.
+
+Import Notations.
+Open Scope monad_scope.
+
+(** ** Functor, Applicative, and Monad Laws *)
+Class Functor_Correct (f : Type -> Type) `{F : Functor f} :=
+  { fmap_id      : forall {A}, fmap (fun (x:A)=> x) = (fun x => x);
+    fmap_compose : forall {A B C} (g : A -> B) (f : B -> C), 
+        fmap (f ∘ g) = fmap f ∘ fmap g
+  }.
+Class Applicative_Correct (f : Type -> Type) `{Applicative f} :=
+{ applicative_id : forall A, liftA (pure (fun  (x:A) => x)) = (fun  x => x);
+  applicative_composition : forall {A B C} (u : f (B -> C)) (v : f (A -> B)) (w : f A),
+    pure (fun  x => fun  y => x ∘ y) <*> u <*> v <*> w = u <*> (v <*> w);
+  applicative_homomorphism : forall {A B} (f : A -> B) (x : A),
+    pure f <*> pure x = pure (f x);
+  applicative_interchange : forall {A B} (u : f (A -> B)) (y : A),
+    u <*> pure y = pure (fun x => x y) <*> u
+}.
+
+Class Monad_Correct (m : Type -> Type) `{M : Monad m} := {
+  bind_right_unit: forall A (a: m A), a = a >>= return_;
+  bind_left_unit: forall A (a: A) B (f: A -> m B),
+             f a = return_ a >>= f;
+  bind_associativity: forall A (ma: m A) B f C (g: B -> m C),
+                 bind ma (fun  x=> f x >>= g) = (ma >>= f) >>= g
+}.
+
+Arguments Functor f : assert.
+Arguments Functor_Correct f {F}.
+Arguments Applicative f [F]. 
+Arguments Applicative_Correct f {F} {A} : rename.
+Arguments Monad m [F] [M].
+Arguments Monad_Correct m [F] [A] [M] : rename.
+
+
+(** ** Helper functions *)
+Section monadic_functions.
+  Context (m : Type -> Type)
+          `{Functor m}
+          `{Applicative m}
+          `{Monad m}.
+ 
+   Definition wbind {A: Type} (ma: m A) {B: Type} (mb: m B) :=
+   ma >>= fun  _=>mb.
+
+   Definition liftM {A B: Type} (f: A->B) (ma: m A): m B :=
+   ma >>= (fun  a => return_ (f a)).
+
+   Definition join {A: Type} (mma: m (m A)): m A :=
+   mma >>= (fun  ma => ma).
+
+  Fixpoint foldM {A B}
+                 (f : B -> A -> m B) (b : B) (ls : list A) : m B :=
+    match ls with
+    | nil      => return_ b
+    | x :: ls' => do y ← f b x;
+                  foldM f y ls'
+    end.
+End monadic_functions.
+
+Section monadic_proofs.
+  Lemma fmap_compose' {f} (F : Functor f) `{Functor_Correct f} : 
+    forall {A B C} (g : A -> B) (h : B -> C) (a : f A),
+    fmap h (fmap g a) = fmap (h ∘ g) a.
+  Proof.
+    intros.
+    rewrite (fmap_compose g h).
+    reflexivity.
+  Qed.
+
+  Lemma bind_eq : forall {A B m} `{Monad m} (a a' : m A) (f f' : A -> m B),
+      a = a' ->
+      (forall x, f x = f' x) ->
+      bind a f = bind a' f'.
+  Proof.
+    intros. subst.
+    f_equal.
+    apply functional_extensionality.
+    auto.
+  Qed.
+End monadic_proofs.
+
+
+(** ** Tactics *)
+Module Tactics.
+
+  Hint Transparent return_.
+
+  (** Reduce by monad laws inside of a goal *)
+ Ltac simplify_monad :=
+  repeat match goal with
+  | [ |- context[ Some ?e ] ] => 
+    let tp := type of e in 
+    replace (Some e) with (return_ e : option tp)
+    by reflexivity
+  | [ |- context[ bind (return_ _) _ ] ] => rewrite <- bind_left_unit
+  | [ |- context[ bind (bind _ _) _ ] ]  => rewrite <- bind_associativity
+  | [ |- _ = _ ]                  => reflexivity
+  | [ |- bind ?a ?f = _ ] => erewrite (bind_eq a);
+                             [ reflexivity | intro; simplify_monad | ]
+  end.
+
+  Ltac simplify_under_monad :=
+    repeat (try match goal with
+    [ |- bind ?a _ = bind ?a _ ] => apply bind_eq; [ reflexivity | intros ]
+    end; simplify_monad).
+End Tactics.
+
+(** * Some classic Monads *)
+
+Module Instances.
+
+(** ** The list monad *)
+
+Open Scope list_scope.
+Definition list_fmap {A B : Type} := @map A B.
+Definition list_liftA {A B} (fs : list (A -> B)) (xs : list A) : list B :=
+  let g := fun a => list_fmap (fun f => f a) fs
+  in concat (list_fmap g xs).
+Fixpoint list_bind {A} (xs : list A) {B} (f : A -> list B) : list B :=
+  match xs with
+  | nil => nil
+  | a :: xs' => f a ++ list_bind xs' f
+  end.
+
+Instance listF : Functor list := { fmap := @list_fmap }.
+Instance listA : Applicative list := { pure := fun _ x => x :: nil
+                                     ; liftA := @list_liftA }.
+Instance listM : Monad list := 
+  { bind := @list_bind }.
+
+Instance listF_correct : Functor_Correct list.
+Proof.
+  constructor.
+  * intros. simpl. apply functional_extensionality; intros x.
+    induction x; simpl; auto.
+    rewrite IHx; auto.
+  * intros. simpl. apply functional_extensionality; intros x.
+    induction x; simpl; auto.
+    rewrite IHx.
+    auto.
+Qed.
+
+Instance listA_correct : Applicative_Correct list.
+Proof.
+  constructor.
+  * intros. simpl. apply functional_extensionality; intros l.
+    induction l; simpl; auto.
+    unfold list_liftA in *. simpl in *.
+    rewrite IHl; easy.
+Abort.
+
+Instance listM_correct : Monad_Correct list.
+Abort.
+
+Lemma fmap_app : forall {A B} (f : A -> B) ls1 ls2,
+      fmap f (ls1 ++ ls2) = fmap f ls1 ++ fmap f ls2.
+Proof.
+  induction ls1; intros; simpl; auto.
+  rewrite IHls1. auto.
+Qed.
+
+(** ** The option monad *)
+
+Definition option_fmap {A B} (f : A -> B) (x : option A) : option B :=
+  match x with
+  | None => None
+  | Some a => Some (f a)
+  end.
+Definition option_liftA {A B} (f : option (A -> B)) (x : option A) : option B :=
+  match f, x with
+  | Some f', Some a => Some (f' a)
+  | _, _ => None
+  end.
+Instance optionF : Functor option := { fmap := @option_fmap}.
+Instance optionA : Applicative option := { pure := @Some;
+                                           liftA := @option_liftA}.
+Instance optionM : Monad option :=
+  { bind := fun  A m B f => match m with None => None | Some a => f a end
+  }.
+Instance optionF_Laws : Functor_Correct option.
+Proof. split.
+  - intros A.
+    apply functional_extensionality; intros op.
+    destruct op; reflexivity.
+  - intros A B C g f.
+    apply functional_extensionality; intros op.
+    destruct op; reflexivity.
+Defined.
+Instance optionA_Laws : Applicative_Correct option.
+Proof. split.
+  - intros A.
+    apply functional_extensionality; intros op.
+    destruct op; reflexivity.
+  - intros A B C [f|] [g|] [a|]; reflexivity.
+  - intros A B f x. reflexivity.
+  - intros A B [f|] a; reflexivity.
+Defined.
+    
+Instance optionM_Laws : Monad_Correct option.
+Proof. split.
+  - destruct a; auto.
+  - intros; auto.
+  - destruct ma; intros; auto.
+Defined.
+
+(** ** Monad Transformers *)
+Class MonadTrans (t : (Type -> Type) -> (Type -> Type)) :=
+  { liftT : forall {m} `{Monad m} {A}, m A -> t m A }.
+
+
+(** Option monad transformer *)
+Definition optionT m (A : Type) : Type := m (option A).
+
+Definition optionT_liftT {m} `{Monad m} {A} (x : m A) : optionT m A.
+Proof.
+  unfold optionT.
+  refine (do a ← x; return_ (Some a)).
+Defined.
+Instance optionT_T : MonadTrans optionT := {liftT := @optionT_liftT}.
+
+Definition optionT_fmap {f} `{Functor f} 
+                        {A B} (g : A -> B) (x : optionT f A) : optionT f B :=
+  @fmap f _ _ _ (fmap g) x.
+Definition optionT_liftA {f} `{Applicative f}
+                         {A B} (g : optionT f (A -> B)) (x : optionT f A) 
+                       : optionT f B.
+(*  @liftA f _ _ _ _ (fmap liftA g) x.*)
+Proof. 
+  unfold optionT in *.
+  exact (fmap liftA g <*> x).
+Defined. 
+Definition optionT_pure {f} `{Applicative f}
+                        {A} (a : A) : optionT f A := @pure f _ _ _ (pure a).
+Definition optionT_bind {m} `{Monad m}
+                        {A} (ma : optionT m A) {B} (f : A -> optionT m B)
+                        : optionT m B.
+  unfold optionT in *.
+  exact (do oa ← ma; 
+         match oa with
+         | None => pure None
+         | Some a => f a
+         end
+  ).
+Defined.
+
+Instance optionT_F {f} `{Functor f} : Functor (optionT f) := 
+    {fmap := @optionT_fmap f _}.
+Instance optionT_A {f} `{Applicative f} : Applicative (optionT f) :=
+  { pure := @optionT_pure f _ _;
+    liftA := @optionT_liftA f _ _ }.
+Instance optionT_M {m} `{Monad m} : Monad (optionT m) :=
+  { bind := @optionT_bind m _ _ _ }.
+
+(** The Reader monad *)
+Axiom Eta: forall A (B: A -> Type) (f: forall a, B a), f = fun  a=>f a.
+
+Definition Reader (E : Type) := fun  X => E -> X.
+Definition reader_fmap E A B (f : A -> B) (r : Reader E A) : Reader E B :=
+  fun x => f (r x).
+Definition reader_liftA E A B (f : Reader E (A -> B)) (r : Reader E A) :=
+  fun x => (f x) (r x).
+Definition reader_bind E A (r : Reader E A) B (f : A -> Reader E B) : Reader E B :=
+  fun x => f (r x) x.
+  
+Instance readerF E : Functor (Reader E) :=
+ { fmap := @reader_fmap E }.
+Instance readerA E : Applicative (Reader E) :=
+ { pure := fun  A (a:A) e=> a;
+   liftA := @reader_liftA E }.
+Instance readerM (E : Type): Monad (Reader E) :=
+ { bind := @reader_bind E }.
+(*
+(* Checking the 3 laws *)
+ - (* unit_left *)
+   intros; apply Eta.
+ - (* unit_right *)
+   intros; apply Eta.
+ - (* associativity *)
+   reflexivity.
+Defined.
+*)
+(** ** The State monad *)
+
+Section State.
+(*Axiom Ext: forall A (B: A->Type) (f g: forall a, B a), (forall a, f a = g a) -> f = g.*)
+
+  Variable S : Type.
+
+  Definition State (A : Type) := S -> A * S.
+  Definition state_fmap A B (f : A -> B) (st : State A) : State B :=
+    fun  s => let (a,s) := st s in (f a,s).
+  Definition state_liftA A B (st_f : State (A -> B)) (st_a : State A) :=
+    fun  s => let (f,s) := st_f s in
+              let (a,s) := st_a s in
+              (f a,s).
+  Definition state_bind A (st_a : State A) B  (f : A -> State B) :=
+    fun  s => let (a,s) := st_a s in
+              f a s.
+
+  Definition put (x : S) : State () :=
+    fun _ => (tt,x).
+  Definition get : State S :=
+    fun x => (x,x).
+  Definition runState  {A} (op : State A) : S -> A * S := op.
+  Definition evalState {A} (op : State A) : S -> A := fst ∘ op.
+  Definition execState {A} (op : State A) : S -> S := snd ∘ op.
+
+
+
+End State.
+Ltac fold_evalState :=
+  match goal with
+  | [ |- context[fst (?c ?v)] ] => replace (fst (c v)) with (evalState c v)
+                                                       by reflexivity
+  end.
+
+Arguments get {S}.
+Arguments put {S}.
+
+Instance stateF {A} : Functor (State A) :=
+    { fmap := @state_fmap A }.
+Instance stateA {A} : Applicative (State A) :=
+    { pure := fun  A a s=> (a,s);
+      liftA := @state_liftA A }.
+Instance stateM {A} : Monad (State A) :=
+    { bind := @state_bind A }.
+
+
+Instance stateF_correct {A} : Functor_Correct (State A).
+  Proof.
+    split; intros;
+      apply functional_extensionality; intros op;
+      apply functional_extensionality; intros x;
+      simpl; unfold state_fmap.
+    - destruct (op x); reflexivity.
+    - destruct (op x); reflexivity.
+  Qed.
+
+Instance stateA_correct {A} : Applicative_Correct (State A).
+  Proof. 
+    split; intros;
+      apply functional_extensionality; intros op; 
+      simpl; unfold state_liftA.
+    - apply functional_extensionality; intros x.
+      destruct (op x); reflexivity.
+    - destruct (u op).
+      destruct (v a).
+      destruct (w a0).
+      reflexivity.
+    - reflexivity.
+    - destruct (u op). 
+      reflexivity.
+  Qed.
+
+Instance stateM_correct {A} : Monad_Correct (State A).
+  Proof.
+    split; intros; simpl; unfold state_bind.
+    - apply functional_extensionality; intros x. 
+      destruct (a x); reflexivity.
+    - reflexivity.
+    - apply functional_extensionality; intros x.
+      destruct (ma x).
+      reflexivity.
+  Qed.
+
+
+End Instances.
